Began preparation for downgrade theorems...

LogicalRefinement/Stlc/Irrel.lean
@@ -17,6 +17,13 @@ open AnnotSort
   | natrec _ n z s, i => n.has_dep i ∨ z.has_dep i ∨ s.has_dep (i + 2)
   | _, _ => False
 
+@[simp] def Stlc.Context.eq_at:  
+  (Γ Δ: Stlc.Context) -> Nat -> Prop
+  | [], [], _ => True
+  | (A::_), (B::_), 0 => A = B
+  | (_::Γ), (_::Δ), n + 1 => eq_at Γ Δ n
+  | _, _, _ => False
+
 @[simp] def Stlc.Context.interp.eq_at:  
   {Γ Δ: Stlc.Context} -> (G: Γ.interp) -> (D: Δ.interp) -> Nat -> Prop
   | [], [], (), (), _ => True
@@ -24,7 +31,26 @@ open AnnotSort
   | (_::_), (_::_), (_, G), (_, G'), n + 1 => G.eq_at G' n
   | _, _, _, _, _ => False
 
-@[simp] def Stlc.Context.interp.eq_at_refl  
+theorem Stlc.Context.interp.eq_at.ctx_eq_at 
+  {Γ Δ: Stlc.Context} {G: Γ.interp} {D: Δ.interp} {n: Nat}
+  (H: G.eq_at D n)
+  : Γ.eq_at Δ n
+  := by {
+    induction n generalizing Γ Δ with
+    | zero => 
+      cases Γ with
+      | nil => cases Δ <;> cases H <;> simp
+      | cons A Γ => cases Δ <;> cases H <;> assumption
+    | succ n I => 
+      cases Γ with
+      | nil => cases Δ <;> cases H <;> simp
+      | cons A Γ => 
+        cases Δ with
+        | nil => cases H
+        | cons => exact I H
+  }
+
+theorem Stlc.Context.interp.eq_at_refl  
   {Γ: Stlc.Context} (G: Γ.interp) (n: Nat):
   G.eq_at G n
   := by {
@@ -36,9 +62,62 @@ open AnnotSort
       | succ n => exact I _ _
   }
 
+theorem Stlc.Context.eq_at_refl  
+  (Γ: Stlc.Context) (n: Nat):
+  Γ.eq_at Γ n
+  := by {
+    induction Γ generalizing n with
+    | nil => exact True.intro
+    | cons H Γ I =>
+      cases n with
+      | zero => rfl
+      | succ n => exact I n
+  }
+
+theorem Stlc.Context.eq_at.symm 
+  {Γ Δ: Stlc.Context} {n}
+  (H: Γ.eq_at Δ n): Δ.eq_at Γ n
+  := by {
+    sorry
+  }
+
+def Stlc.Context.eq_mod 
+  (Γ Δ: Stlc.Context) (a: Stlc): Prop
+  := ∀n: Nat, a.has_dep n -> Γ.eq_at Δ n
+
 def Stlc.Context.interp.eq_mod 
   {Γ Δ: Stlc.Context} (G: Γ.interp) (D: Δ.interp) (a: Stlc): Prop
   := ∀n: Nat, a.has_dep n -> G.eq_at D n
+
+theorem Stlc.Context.interp.eq_mod.ctx_eq_mod 
+  {Γ Δ: Stlc.Context} {G: Γ.interp} {D: Δ.interp} {a: Stlc}
+  (H: G.eq_mod D a)
+  : Γ.eq_mod Δ a
+  := λn Hd => (H n Hd).ctx_eq_at
+
+theorem Stlc.Context.eq_mod.symm 
+  {Γ Δ: Stlc.Context} {a}
+  (H: Γ.eq_mod Δ a): Δ.eq_mod Γ a
+  := by {
+    sorry
+  }
+
+--TODO: var theorems
+
+theorem Stlc.Context.eq_mod.deriv
+  {Γ Δ: Stlc.Context} {a: Stlc} {A: Ty} 
+  (H: Γ.eq_mod Δ a)
+  (HΓ: Γ ⊧ a: A)
+  : (Δ ⊧ a: A)
+  := by {
+    sorry
+  }
+
+theorem Stlc.Context.eq_mod.deriv_eq
+  {Γ Δ: Stlc.Context} {a: Stlc} {A: Ty} 
+  (H: Γ.eq_mod Δ a)
+  : (Γ ⊧ a: A) = (Δ ⊧ a: A)
+  := propext (Iff.intro (λHΓ => H.deriv HΓ) (λHΔ => H.symm.deriv HΔ))
 
 theorem Stlc.HasVar.interp_eq_mod
   {Γ Δ: Stlc.Context} {n: Nat} {A: Ty} {G: Γ.interp} {D: Δ.interp}
